Rework environments

src/MicroSail.v
@@ -1,7 +1,9 @@
-Require Export Coq.Unicode.Utf8.
-Require Import Coq.ZArith.ZArith.
-Require Import Coq.Strings.String.
-Require Import Coq.Program.Tactics.
+From Coq Require Import
+     Logic.EqdepFacts
+     Program.Equality
+     Program.Tactics
+     Strings.String
+     ZArith.ZArith.
 
 Set Implicit Arguments.
 
@@ -20,83 +22,193 @@ Section Contexts.
     | ctx_snoc Γ₂ τ => ctx_snoc (ctx_cat Γ₁ Γ₂) τ
     end.
 
-  Fixpoint ctx_nth {B : Set} (Γ : Ctx B) (n : nat) {struct Γ} : option B :=
+  (* Fixpoint ctx_nth {B : Set} (Γ : Ctx B) (n : nat) {struct Γ} : option B := *)
+  (*   match Γ , n with *)
+  (*   | ctx_snoc _ x , O   => Some x *)
+  (*   | ctx_snoc Γ _ , S n => ctx_nth Γ n *)
+  (*   | _            , _   => None *)
+  (*   end. *)
+
+  Fixpoint ctx_nth_is {B : Set} (Γ : Ctx B) (n : nat) (b : B) {struct Γ} : Prop :=
     match Γ , n with
-    | ctx_snoc _ x , O   => Some x
-    | ctx_snoc Γ _ , S n => ctx_nth Γ n
-    | _            , _   => None
+    | ctx_snoc _ x , O   => x = b
+    | ctx_snoc Γ _ , S n => ctx_nth_is Γ n b
+    | _            , _   => False
     end.
 
+  (* InCtx represents context containment proofs. This is essentially a
+     well-typed de Bruijn index, i.e. a de Bruijn index with a proof that it
+     resolves to the binding b.
+     SK: I wanted to play with a sigma type here instead of using some unary
+     representation. There might be some headaches in proofs ahead which require
+     eta for sig which is AFAIK not given definitionally only propositionally.
+     For instance proving that lookup and tabulation are inverses requires eta.
+     this. *)
   Class InCtx {B : Set} (b : B) (Γ : Ctx B) : Set :=
-    inCtx : { n : nat | ctx_nth Γ n = Some b }.
+    inCtx : { n : nat | ctx_nth_is Γ n b }.
 
   Definition inctx_zero {B : Set} {b : B} {Γ : Ctx B} : InCtx b (ctx_snoc Γ b) :=
     exist _ 0 eq_refl.
   Definition inctx_succ {B : Set} {b : B} {Γ : Ctx B} {b' : B} (bIn : InCtx b Γ) :
-    InCtx b (ctx_snoc Γ b') := let (n, e) := bIn in exist _ (S n) e.
+    InCtx b (ctx_snoc Γ b') := exist _ (S (proj1_sig bIn)) (proj2_sig bIn).
+
+  (* Custom pattern matching in cases where the context was already refined
+     by a different match, i.e. on environments. *)
+  Definition inctx_case_nil {A B : Set} {x : B} (xIn : InCtx x ctx_nil) : A :=
+    let (n, e) := xIn in match e with end.
+  Definition inctx_case_snoc (X : Set) (D : X -> Set) (Γ : Ctx X) (x : X) (dx : D x)
+    (dΓ: forall z, InCtx z Γ -> D z) (y: X) (yIn: InCtx y (ctx_snoc Γ x)) : D y :=
+    let (n, e) := yIn in
+    match n return (ctx_nth_is (ctx_snoc Γ x) n y -> D y) with
+    | 0 =>   eq_rec x D dx y
+    | S n => fun e => dΓ y (exist _ n e)
+    end e.
+
+  Definition inctx_case_snoc_dep (X : Set) (Γ : Ctx X) (x : X)
+    (D : forall z, InCtx z (ctx_snoc Γ x) -> Prop)
+    (dx : D x inctx_zero)
+    (dΓ: forall z (zIn: InCtx z Γ), D z (inctx_succ zIn)) :
+    forall (y: X) (yIn: InCtx y (ctx_snoc Γ x)), D y yIn :=
+    fun y yIn =>
+      match yIn with
+        exist _ n e =>
+        match n return (forall e, D y (exist _ n e)) with
+        | 0 => fun e => eq_indd X x (fun z e => D z (exist _ 0 e)) dx y e
+        | S n => fun e => dΓ y (exist (fun n => ctx_nth_is Γ n y) n e)
+        end e
+      end.
 
 End Contexts.
 
 Section Environments.
 
-  Definition Env {X T : Set} (D : T -> Set) (Γ : Ctx (X * T)) : Set :=
-    forall (x : X) (τ : T), InCtx (x,τ) Γ -> D τ.
+  Context {X : Set}.
 
-  Definition env_nil {X T : Set} {D : T -> Set} : @Env X T D ctx_nil :=
-    fun x τ xIn => let (n, e) := xIn in
-    eq_rec None (fun m => match m with | Some _ => D τ | None => unit end) tt (Some (x, τ)) e.
+  Inductive Env (D : X -> Set) : Ctx X -> Set :=
+  | env_nil : Env D ctx_nil
+  | env_snoc {Γ} (E : Env D Γ) (x : X) (d : D x) :
+      Env D (ctx_snoc Γ x).
 
-  Definition env_snoc {X T : Set} {D : T -> Set} {Γ : Ctx (X * T)}
-             (E : Env D Γ) (x : X) (τ : T) (d : D τ) : Env D (ctx_snoc Γ (x , τ)).
-  Admitted.
+  Global Arguments env_nil {_}.
 
-  Definition env_cat {X T : Set} {D : T -> Set} {Γ Δ : Ctx (X * T)}
-             (EΓ : Env D Γ) (EΔ : Env D Δ) : Env D (ctx_cat Γ Δ).
-  Admitted.
+  Fixpoint env_cat {D : X -> Set} {Γ Δ : Ctx X}
+           (EΓ : Env D Γ) (EΔ : Env D Δ) : Env D (ctx_cat Γ Δ) :=
+    match EΔ with
+    | env_nil => EΓ
+    | env_snoc E x d => env_snoc (env_cat EΓ E) x d
+    end.
 
-  (* Definition env_nil {X T : Set} {D : T -> Set} : @Env X T D ctx_nil := *)
-  (*   fun y σ yIn => *)
-  (*     match yIn in InCtx _ Γx *)
-  (*               return match Γx with *)
-  (*                      | ctx_nil => D σ *)
-  (*                      | ctx_snoc _ _ => unit *)
-  (*                      end *)
-  (*               with *)
-  (*               | inctx_zero _ => tt *)
-  (*               | inctx_succ i => tt *)
-  (*     end. *)
+  Fixpoint env_map {D₁ D₂ : X -> Set} {Γ : Ctx X}
+    (f : forall x, D₁ x -> D₂ x) (E : Env D₁ Γ) : Env D₂ Γ :=
+    match E with
+    | env_nil => env_nil
+    | env_snoc E x d => env_snoc (env_map f E) x (f x d)
+    end.
 
-  (* Definition env_snoc {X T : Set} {D : T -> Set} {Γ : Ctx (X * T)} *)
-  (*   (E : Env D Γ) (x : X) (τ : T) (d : D τ) : Env D (ctx_snoc Γ (x , τ)) := *)
-  (*   fun y σ yIn => match yIn in InCtx _ Γx *)
-  (*               return match Γx with *)
-  (*                      | ctx_nil => Empty_set *)
-  (*                      | ctx_snoc Γ (_, τ) => Env D Γ -> D τ -> D σ *)
-  (*                      end *)
-  (*               with *)
-  (*               | inctx_zero _ => λ _ d, d *)
-  (*               | @inctx_succ _ _ _ (_ , _) i => fun E _ => E y σ i *)
-  (*               end E d. *)
+  Fixpoint env_lookup {D : X -> Set} {Γ : Ctx X}
+           (E : Env D Γ) : forall (x : X) (i : InCtx x Γ), D x :=
+    match E with
+    | env_nil => fun _ => inctx_case_nil
+    | env_snoc E x d => inctx_case_snoc D d (env_lookup E)
+    end.
 
-  Global Arguments env_snoc {_ _ _ _} _ _ _ _.
+  Arguments env_lookup {_ _} _ [_] _.
 
-  Definition env_drop {X T : Set} {D : T -> Set} {Γ : Ctx (X * T)}
-    (x : X) (τ : T) (E : Env D (ctx_snoc Γ (x , τ))) : Env D Γ :=
-    fun y σ yIn => E y σ (inctx_succ yIn).
+  Fixpoint env_update {D : X -> Set} {Γ : Ctx X} (E : Env D Γ) {struct E} :
+    forall {x : X} (i : InCtx x Γ) (d : D x), Env D Γ :=
+    match E with
+    | env_nil => fun _ => inctx_case_nil
+    | @env_snoc _ Γ E y old =>
+      inctx_case_snoc
+        (fun x => D x -> Env D (ctx_snoc Γ y))
+        (fun new => env_snoc E y new)
+        (fun x xIn new => env_snoc (env_update E xIn new) y old)
+    end.
 
-  Definition env_map {X T : Set} {D₁ D₂ : T -> Set} {Γ : Ctx (X * T)}
-    (f : forall τ, D₁ τ -> D₂ τ) (E : Env D₁ Γ) : Env D₂ Γ :=
-    fun y σ yIn => f _ (E y σ yIn).
-  Definition env_lookup {X T : Set} {D : T -> Set} {Γ : Ctx (X * T)}
-    (E : Env D Γ) {x : X} {τ : T} (i : InCtx (x , τ) Γ) : D τ := E _ _ i.
-  Definition env_update {X T : Set} {D : T -> Set} {Γ : Ctx (X * T)}
-    (E : Env D Γ) {x : X} {τ : T} (i : InCtx (x , τ) Γ) (d : D τ) : Env D Γ.
-  Admitted.
+  Definition env_tail {D : X -> Set} {Γ : Ctx X}
+    {x : X} (E : Env D (ctx_snoc Γ x)) : Env D Γ :=
+    match E in Env _ Γx
+    return match Γx with
+           | ctx_nil => unit
+           | ctx_snoc Γ _ => Env D Γ
+           end
+    with
+      | env_nil => tt
+      | env_snoc E _ _ => E
+    end.
+
+  Global Arguments env_tail {_ _ _} / _.
+
+  Fixpoint env_drop {D : X -> Set} {Γ : Ctx X} Δ {struct Δ} :
+    forall (E : Env D (ctx_cat Γ Δ)), Env D Γ :=
+    match Δ with
+    | ctx_nil => fun E => E
+    | ctx_snoc Δ _ => fun E => env_drop Δ (env_tail E)
+    end.
+
+  Fixpoint env_split {D : X -> Set} {Γ : Ctx X} Δ {struct Δ} :
+    forall (E : Env D (ctx_cat Γ Δ)), Env D Γ * Env D Δ :=
+    match Δ with
+    | ctx_nil => fun E => (E , env_nil)
+    | ctx_snoc Δ b =>
+      fun E =>
+        match E in (Env _ ΓΔx)
+        return match ΓΔx with
+               | ctx_nil => unit
+               | ctx_snoc ΓΔ x => (Env D ΓΔ -> Env D Γ * Env D Δ) ->
+                                  Env D Γ * Env D (ctx_snoc Δ x)
+               end
+        with
+        | env_nil => tt
+        | env_snoc EΓΔ x d =>
+          fun split => let (EΓ, EΔ) := split EΓΔ in (EΓ, env_snoc EΔ x d)
+        end (env_split Δ)
+    end.
+
+  Lemma env_lookup_update {D : X -> Set} {Γ : Ctx X} (E : Env D Γ) :
+    forall {x:X} (xInΓ : InCtx x Γ) (d : D x),
+      env_lookup (env_update E xInΓ d) xInΓ = d.
+  Proof.
+    induction E; intros y [n e]; try destruct e;
+      destruct n; cbn in *; subst; auto.
+  Qed.
+
+  Lemma env_split_cat {D : X -> Set} {Γ Δ : Ctx X} :
+    forall (EΓ : Env D Γ) (EΔ : Env D Δ),
+      env_split Δ (env_cat EΓ EΔ) = (EΓ , EΔ).
+  Proof. induction EΔ using Env_ind; cbn; now try rewrite IHEΔ. Qed.
+
+  Lemma env_cat_split' {D : X -> Set} {Γ Δ : Ctx X} :
+    forall (EΓΔ : Env D (ctx_cat Γ Δ)),
+      let (EΓ,EΔ) := env_split _ EΓΔ in
+      EΓΔ = env_cat EΓ EΔ.
+  Proof.
+    induction Δ; intros; cbn in *.
+    - reflexivity.
+    - dependent destruction EΓΔ.
+      specialize (IHΔ EΓΔ); cbn in *.
+      destruct (env_split Δ EΓΔ); now subst.
+  Qed.
+
+  Lemma env_cat_split {D : X -> Set} {Γ Δ : Ctx X} (EΓΔ : Env D (ctx_cat Γ Δ)) :
+    EΓΔ = env_cat (fst (env_split _ EΓΔ)) (snd (env_split _ EΓΔ)).
+  Proof.
+    generalize (env_cat_split' EΓΔ).
+    now destruct (env_split Δ EΓΔ).
+  Qed.
+
+  Lemma env_drop_cat {D : X -> Set} {Γ Δ : Ctx X} :
+    forall (δΔ : Env D Δ) (δΓ : Env D Γ),
+      env_drop Δ (env_cat δΓ δΔ) = δΓ.
+  Proof. induction δΔ; cbn; auto. Qed.
 
 End Environments.
 
 (* Section Types. *)
 Module Type TypeKit.
+
+  Definition Env' {X T : Set} (D : T -> Set) (Γ : Ctx (X * T)) : Set :=
+    Env (fun xt => D (snd xt)) Γ.
 
   (* Names of union type constructors. *)
   Parameter 𝑻   : Set. (* input: \MIT *)
@@ -129,9 +241,9 @@ Module Type TypeKit.
     Notation "Γ ▻ b" := (ctx_snoc Γ b) (at level 55, left associativity).
     Notation "Γ₁ ▻▻ Γ₂" := (ctx_cat Γ₁ Γ₂) (at level 55, left associativity).
     Notation "b ∈ Γ" := (InCtx b Γ)  (at level 80).
-    Notation "E '►' x '∶' τ '↦' d" := (env_snoc E x τ d) (at level 55, left associativity).
+    Notation "E '►' x '∶' τ '↦' d" := (E , ((x , τ) , d)) (at level 55, left associativity).
     Notation "E1 '►►' E2" := (env_cat E1 E2) (at level 55, left associativity).
-    Notation "E [ x ↦ v ]" := (@env_update _ _ _ _ E x _ _ v) (at level 55, left associativity).
+    Notation "E [ x ↦ v ]" := (@env_update _ _ _ E (x , _) _ v) (at level 55, left associativity).
 
   End NameNotation.
 
@@ -168,7 +280,7 @@ Module Type TermKit (typeKit : TypeKit).
     | taglit_sum    σ₁ σ₂  : TaggedLit σ₁ + TaggedLit σ₂ -> TaggedLit (ty_sum σ₁ σ₂)
     | taglit_unit          : TaggedLit (ty_unit)
     | taglit_union (T : 𝑻) (K : 𝑲 T) : TaggedLit (𝑲_Ty K) -> TaggedLit (ty_union T)
-    | taglit_record (R : 𝑹) : Env TaggedLit (𝑹𝑭_Ty R) -> TaggedLit (ty_record R).
+    | taglit_record (R : 𝑹) : Env' TaggedLit (𝑹𝑭_Ty R) -> TaggedLit (ty_record R).
 
     Fixpoint Lit (σ : Ty) : Set :=
       match σ with
@@ -181,12 +293,12 @@ Module Type TermKit (typeKit : TypeKit).
       | ty_sum σ₁ σ₂ => Lit σ₁ + Lit σ₂
       | ty_unit => unit
       | ty_union T => { K : 𝑲 T & TaggedLit (𝑲_Ty K) }
-      | ty_record R => Env TaggedLit (𝑹𝑭_Ty R)
+      | ty_record R => Env' TaggedLit (𝑹𝑭_Ty R)
       end%type.
 
     Fixpoint untag {σ : Ty} (v : TaggedLit σ) : Lit σ :=
       match v with
-      | taglit_int  z       => z
+      | taglit_int z        => z
       | taglit_bool b       => b
       | taglit_bit b        => b
       | taglit_string s     => s
@@ -199,7 +311,7 @@ Module Type TermKit (typeKit : TypeKit).
       | taglit_record t     => t
       end.
 
-    Definition LocalStore (Γ : Ctx (𝑿 * Ty)) : Set := Env Lit Γ.
+    Definition LocalStore (Γ : Ctx (𝑿 * Ty)) : Set := Env' Lit Γ.
 
   End Literals.
 
@@ -224,7 +336,7 @@ Module Type TermKit (typeKit : TypeKit).
     | exp_cons    {σ : Ty} (h : Exp Γ σ) (t : Exp Γ (ty_list σ)) : Exp Γ (ty_list σ)
     | exp_nil     {σ : Ty} : Exp Γ (ty_list σ)
     | exp_union   {T : 𝑻} (K : 𝑲 T) (e : Exp Γ (𝑲_Ty K)) : Exp Γ (ty_union T)
-    | exp_record  (R : 𝑹) (es : Env (Exp Γ) (𝑹𝑭_Ty R)) : Exp Γ (ty_record R)
+    | exp_record  (R : 𝑹) (es : Env' (Exp Γ) (𝑹𝑭_Ty R)) : Exp Γ (ty_record R)
     | exp_builtin {σ τ : Ty} (f : Lit σ -> Lit τ) (e : Exp Γ σ) : Exp Γ τ.
 
     Global Arguments exp_union {_ _} _ _.
@@ -257,6 +369,9 @@ Module Type TermKit (typeKit : TypeKit).
       | exp_builtin f e     => f (eval e δ)
       end.
 
+    Definition evals {Γ Δ} (es : Env' (Exp Γ) Δ) (δ : LocalStore Γ) : LocalStore Δ :=
+      env_map (fun xτ e => eval e δ) es.
+
   End Expressions.
 
   Section Statements.
@@ -274,7 +389,7 @@ Module Type TermKit (typeKit : TypeKit).
     | stm_let        (x : 𝑿) (τ : Ty) (s : Stm Γ τ) {σ : Ty} (k : Stm (ctx_snoc Γ (x , τ)) σ) : Stm Γ σ
     | stm_let'       (Δ : Ctx (𝑿 * Ty)) (δ : LocalStore Δ) {σ : Ty} (k : Stm (ctx_cat Γ Δ) σ) : Stm Γ σ
     | stm_assign     (x : 𝑿) (τ : Ty) {xInΓ : InCtx (x , τ) Γ} (e : Exp Γ τ) : Stm Γ τ
-    | stm_app        (f : 𝑭) (es : Env (Exp Γ) (fun_dom (pi f))) : Stm Γ (fun_cod (pi f))
+    | stm_app        (f : 𝑭) (es : Env' (Exp Γ) (fun_dom (pi f))) : Stm Γ (fun_cod (pi f))
     | stm_app'       (Δ : Ctx (𝑿 * Ty)) (δ : LocalStore Δ) (τ : Ty) (s : Stm Δ τ) : Stm Γ τ
     | stm_if         {τ : Ty} (e : Exp Γ ty_bool) (s₁ s₂ : Stm Γ τ) : Stm Γ τ
     | stm_seq        {τ : Ty} (e : Stm Γ τ) {σ : Ty} (k : Stm Γ σ) : Stm Γ σ
@@ -370,13 +485,14 @@ Module Type ProgramKit (typeKit : TypeKit) (termKit : TermKit typeKit).
   Section SmallStep.
 
     Fixpoint pattern_match {rfs : Ctx (𝑹𝑭 * Ty)}  {Δ : Ctx (𝑿 * Ty)}
-             (p : RecordPat rfs Δ) {struct p} : Env TaggedLit rfs -> LocalStore Δ :=
+             (p : RecordPat rfs Δ) {struct p} : Env' TaggedLit rfs -> LocalStore Δ :=
       match p with
       | pat_nil => fun _ => env_nil
       | pat_cons p rf x =>
-        fun E => env_snoc
-               (pattern_match p (fun rf τ H => E rf τ (inctx_succ H))) x _
-               (untag (E rf _ inctx_zero))
+        fun E =>
+          env_snoc
+            (pattern_match p (env_tail E)) (x, _)
+            (untag (env_lookup E inctx_zero))
       end.
 
     (* Record State (Γ : Ctx (𝑿 * Ty)) (σ : Ty) : Set := *)
@@ -385,37 +501,39 @@ Module Type ProgramKit (typeKit : TypeKit) (termKit : TermKit typeKit).
     (*   }. *)
 
     (* Notation "'⟨' δ ',' s '⟩'" := {| state_local_store := δ; state_statement := s |}. *)
+    (* Reserved Notation "st1 '--->' st2" (at level 80). *)
     Reserved Notation "'⟨' δ1 ',' s1 '⟩' '--->' '⟨' δ2 ',' s2 '⟩'" (at level 80).
 
     Import NameNotation.
 
+    (* Inductive Step {Γ : Ctx (𝑿 * Ty)} : forall {σ : Ty} (st₁ st₂ : State Γ σ), Prop := *)
     Inductive Step {Γ : Ctx (𝑿 * Ty)} : forall {σ : Ty} (δ₁ δ₂ : LocalStore Γ) (s₁ s₂ : Stm Γ σ), Prop :=
 
     | step_stm_exp
         (δ : LocalStore Γ) (σ : Ty) (e : Exp Γ σ) :
         ⟨ δ , stm_exp e ⟩ ---> ⟨ δ , stm_lit σ (eval e δ) ⟩
 
+    | step_stm_let_value
+        (δ : LocalStore Γ) (x : 𝑿) (τ σ : Ty) (v : Lit τ) (k : Stm (Γ ▻ (x , τ)) σ) :
+        ⟨ δ , stm_let x τ (stm_lit τ v) k ⟩ ---> ⟨ δ , stm_let' (env_snoc env_nil (x,τ) v) k ⟩
+    | step_stm_let_exit
+        (δ : LocalStore Γ) (x : 𝑿) (τ σ : Ty) (s : string) (k : Stm (Γ ▻ (x , τ)) σ) :
+        ⟨ δ , stm_let x τ (stm_exit τ s) k ⟩ ---> ⟨ δ , stm_exit σ s ⟩
     | step_stm_let_step
         (δ : LocalStore Γ) (δ' : LocalStore Γ) (x : 𝑿) (τ σ : Ty)
         (s : Stm Γ τ) (s' : Stm Γ τ) (k : Stm (Γ ▻ (x , τ)) σ) :
         ⟨ δ , s ⟩ ---> ⟨ δ' , s' ⟩ ->
         ⟨ δ , stm_let x τ s k ⟩ ---> ⟨ δ' , stm_let x τ s' k ⟩
-    | step_stm_let_value
-        (δ : LocalStore Γ) (x : 𝑿) (τ σ : Ty) (v : Lit τ) (k : Stm (Γ ▻ (x , τ)) σ) :
-        ⟨ δ , stm_let x τ (stm_lit τ v) k ⟩ ---> ⟨ δ , stm_let' (env_nil ► x∶τ ↦ v) k ⟩
-    | step_stm_let_exit
-        (δ : LocalStore Γ) (x : 𝑿) (τ σ : Ty) (s : string) (k : Stm (Γ ▻ (x , τ)) σ) :
-        ⟨ δ , stm_let x τ (stm_exit τ s) k ⟩ ---> ⟨ δ , stm_exit σ s ⟩
-    | step_stm_let'_step
-        (δ δ' : LocalStore Γ) (Δ : Ctx (𝑿 * Ty)) (δΔ δΔ' : LocalStore Δ) (σ : Ty) (k k' : Stm (Γ ▻▻ Δ) σ) :
-        ⟨ δ ►► δΔ , k ⟩ ---> ⟨ δ' ►► δΔ' , k' ⟩ ->
-        ⟨ δ , stm_let' δΔ k ⟩ ---> ⟨ δ' , stm_let' δΔ' k' ⟩
     | step_stm_let'_value
         (δ : LocalStore Γ) (Δ : Ctx (𝑿 * Ty)) (δΔ : LocalStore Δ) (σ : Ty) (v : Lit σ) :
         ⟨ δ , stm_let' δΔ (stm_lit σ v) ⟩ ---> ⟨ δ , stm_lit σ v ⟩
     | step_stm_let'_exit
         (δ : LocalStore Γ) (Δ : Ctx (𝑿 * Ty)) (δΔ : LocalStore Δ) (σ : Ty) (s : string) :
         ⟨ δ , stm_let' δΔ (stm_exit σ s) ⟩ ---> ⟨ δ , stm_exit σ s ⟩
+    | step_stm_let'_step
+        (δ δ' : LocalStore Γ) (Δ : Ctx (𝑿 * Ty)) (δΔ δΔ' : LocalStore Δ) (σ : Ty) (k k' : Stm (Γ ▻▻ Δ) σ) :
+        ⟨ δ ►► δΔ , k ⟩ ---> ⟨ δ' ►► δΔ' , k' ⟩ ->
+        ⟨ δ , stm_let' δΔ k ⟩ ---> ⟨ δ' , stm_let' δΔ' k' ⟩
 
     | step_stm_seq_step
         (δ δ' : LocalStore Γ) (τ σ : Ty) (s s' : Stm Γ τ) (k : Stm Γ σ) :
@@ -433,9 +551,9 @@ Module Type ProgramKit (typeKit : TypeKit) (termKit : TermKit typeKit).
         let Δ := fun_dom (pi f) in
         let τ := fun_cod (pi f) in
         let s := fun_body (Pi f) in
-        forall (es : Env (Exp Γ) Δ),
+        forall (es : Env' (Exp Γ) Δ),
         ⟨ δ , stm_app f es ⟩ --->
-        ⟨ δ , stm_app' Δ (fun x σ xInΔ => eval (es x σ xInΔ) δ) τ s ⟩
+        ⟨ δ , stm_app' Δ (evals es δ) τ s ⟩
     | step_stm_app'_step
         {δ : LocalStore Γ} (Δ : Ctx (𝑿 * Ty)) {δΔ δΔ' : LocalStore Δ} (τ : Ty)
         (s s' : Stm Δ τ) :
@@ -450,7 +568,7 @@ Module Type ProgramKit (typeKit : TypeKit) (termKit : TermKit typeKit).
     | step_stm_assign
         (δ : LocalStore Γ) (x : 𝑿) (σ : Ty) {xInΓ : InCtx (x , σ) Γ} (e : Exp Γ σ) :
         let v := eval e δ in
-        ⟨ δ , stm_assign x e ⟩ ---> ⟨ δ [ x ↦ v ] , stm_lit σ v ⟩
+        ⟨ δ , stm_assign x e ⟩ ---> ⟨ env_update δ xInΓ v , stm_lit σ v ⟩
     | step_stm_if
         (δ : LocalStore Γ) (e : Exp Γ ty_bool) (σ : Ty) (s₁ s₂ : Stm Γ σ) :
         ⟨ δ , stm_if e s₁ s₂ ⟩ ---> ⟨ δ , if eval e δ then s₁ else s₂ ⟩
@@ -468,7 +586,7 @@ Module Type ProgramKit (typeKit : TypeKit) (termKit : TermKit typeKit).
         ⟨ δ , stm_match_list e alt_nil xh xt alt_cons ⟩ --->
         ⟨ δ , match eval e δ with
               | nil => alt_nil
-              | cons vh vt => stm_let' (env_nil ► xh∶σ ↦ vh ► xt∶ty_list σ ↦ vt) alt_cons
+              | cons vh vt => stm_let' (env_snoc (env_snoc env_nil (xh,σ) vh) (xt,ty_list σ) vt) alt_cons
               end
         ⟩
     | step_stm_match_sum
@@ -477,8 +595,8 @@ Module Type ProgramKit (typeKit : TypeKit) (termKit : TermKit typeKit).
         (xinr : 𝑿) (alt_inr : Stm (Γ ▻ (xinr , σinr)) τ) :
         ⟨ δ , stm_match_sum e xinl alt_inl xinr alt_inr ⟩ --->
         ⟨ δ , match eval e δ with
-              | inl v => stm_let' (env_nil ► xinl∶σinl ↦ v) alt_inl
-              | inr v => stm_let' (env_nil ► xinr∶σinr ↦ v) alt_inr
+              | inl v => stm_let' (env_snoc env_nil (xinl,σinl) v) alt_inl
+              | inr v => stm_let' (env_snoc env_nil (xinr,σinr) v) alt_inr
               end
         ⟩
     | step_stm_match_pair
@@ -486,14 +604,14 @@ Module Type ProgramKit (typeKit : TypeKit) (termKit : TermKit typeKit).
         (rhs : Stm (Γ ▻ (xl , σ₁) ▻ (xr , σ₂)) τ) :
         ⟨ δ , stm_match_pair e xl xr rhs ⟩ --->
         ⟨ δ , let (vl , vr) := eval e δ in
-              stm_let' (env_nil ► xl∶σ₁ ↦ vl ► xr∶σ₂ ↦ vr) rhs
+              stm_let' (env_snoc (env_snoc env_nil (xl,σ₁) vl) (xr,σ₂) vr) rhs
         ⟩
     | step_stm_match_union
         (δ : LocalStore Γ) {T : 𝑻} (e : Exp Γ (ty_union T)) {τ : Ty}
         (alts : forall (K : 𝑲 T), { x : 𝑿 & Stm (ctx_snoc Γ (x , 𝑲_Ty K)) τ}) :
         ⟨ δ , stm_match_union e alts ⟩ --->
         ⟨ δ , let (K , v) := eval e δ in
-              stm_let' (env_nil ► projT1 (alts K)∶𝑲_Ty K ↦ untag v) (projT2 (alts K))
+              stm_let' (env_snoc env_nil (projT1 (alts K),𝑲_Ty K) (untag v)) (projT2 (alts K))
         ⟩
     | step_stm_match_record
         (δ : LocalStore Γ) {R : 𝑹} {Δ : Ctx (𝑿 * Ty)}
@@ -502,6 +620,7 @@ Module Type ProgramKit (typeKit : TypeKit) (termKit : TermKit typeKit).
         ⟨ δ , stm_match_record R e p rhs ⟩ --->
         ⟨ δ , stm_let' (pattern_match p (eval e δ)) rhs ⟩
 
+    (* where "st1 '--->' st2" := (@Step _ _ st1 st2). *)
     where "'⟨' δ1 ',' s1 '⟩' '--->' '⟨' δ2 ',' s2 '⟩'" := (@Step _ _ δ1 δ2 s1 s2).
 
     Definition Final {Γ σ} (s : Stm Γ σ) : Prop :=
@@ -513,7 +632,7 @@ Module Type ProgramKit (typeKit : TypeKit) (termKit : TermKit typeKit).
 
     Lemma can_form_store_cat (Γ Δ : Ctx (𝑿 * Ty)) (δ : LocalStore (Γ ▻▻ Δ)) :
       exists (δ₁ : LocalStore Γ) (δ₂ : LocalStore Δ), δ = env_cat δ₁ δ₂.
-    Admitted.
+    Proof. pose (env_cat_split δ); eauto. Qed.
 
     (* Lemma can_form_store_snoc (Γ : Ctx (𝑿 * Ty)) (x : 𝑿) (σ : Ty) (δ : LocalStore (Γ ▻ (x , σ))) : *)
     (*   exists (δ' : LocalStore Γ) (v : Lit σ), δ = env_snoc δ' x σ v. *)
@@ -557,14 +676,14 @@ Module Type ProgramKit (typeKit : TypeKit) (termKit : TermKit typeKit).
 
     Local Ltac progress_tac :=
       progress_simpl;
-      try solve
-          [ repeat eexists; constructor; eauto
-          | progress_inst progress_tac
-          ].
+      solve
+        [ repeat eexists; constructor; eauto
+        | progress_inst progress_tac
+        ].
 
     Lemma progress {Γ σ} (s : Stm Γ σ) :
       Final s \/ forall δ, exists δ' s', ⟨ δ , s ⟩ ---> ⟨ δ' , s' ⟩.
-    Proof. induction s; intros; progress_tac. Qed.
+    Proof. induction s; intros; try progress_tac. Qed.
 
   End SmallStep.
 
